\documentclass[10pt, a4paper]{article}
\usepackage{preamble}

\title{Dynamics I}
\author{Luke Phillips}
\date{January 2025}

\begin{document}

\maketitle

\newpage

\tableofcontents

\newpage

\section{Particle on a line}

\subsection{The Basics}

\begin{definition}[Position]
    The position $x(t)$ where $t$ is time.
\end{definition}

\begin{definition}[Velocity]
    The velocity $\dot{x}(t)$ where $t$ is time.
\end{definition}

\textit{Note that $\dot{x}$ means $\frac{dx}{dt}$.}

\begin{definition}[Acceleration]
    The acceleration $a(t) = \dot{v}(t) = \ddot{x}(t)$.
\end{definition}

\begin{definition}[Speed]
    The speed is $|v(t)|$,
    the magnitude of the velocity.
\end{definition}

\begin{definition}[Mass]
    A particle has mass $m > 0$.
\end{definition}

\begin{definition}[Momentum]
    A particle's momentum,
    $p$ is given by
    \[
    p = mv = m\dot{x}.
    \]
\end{definition}

\begin{definition}[Equation of motion]
    In an applied force $F$,
    then the equation of motion is $\dot{p} = F$.
\end{definition}

\begin{remark}\phantom{}
    \begin{enumerate}[label = (\roman*)]
        \item Could have $m$ depending on time
        (e.g. rocket).

        Unless otherwise stated,
        we take $m$ to be a \textbf{constant}.

        Then the EoM\footnote{Equation of motion} is $m\dot{v} = m\ddot{x} = F$.

        \item In general,
        $F = F(t, x, \dot{x})$ and $m\ddot{x} = F(t, x, \dot{x})$ is a second order differential equation which cannot be solved
        (explicitly).
    \end{enumerate}
\end{remark}

We focus on special cases which can be solved.

The simplest example is $F$ is constant.
For example,
vertical motion under gravity close to the surface of a planet:
then the magnitude of $F$ is $|F| = mg$
(the weight)
where the constant $g$ depends on the planet.

\begin{example}
    An object is shot up vertically from the ground with some initial speed $u$.
    What maximum height $H$ does it reach?
    \begin{solution}
        Could use $x$ upwards or $x$ downwards,
        both work,
        choose a convenient one.
        Here having $x$ upwards seems more natural.
        Then $m\ddot{x} = -mg$ with $x = 0$ at the ground.
        Then
        \begin{align*}
            \ddot{x} = -g &\xrightarrow{\int\,dt} \dot{x} = -gt + u \\
            \intertext{where $u$ is the constant of integration.} \\
            &\xrightarrow{\int\,dt} x(t) = -\frac{1}{2}gt ^ 2 + ut + 0.
        \end{align*}
        Max $\dot{x} = 0 \implies t = u / g$.
        So $H = x\left(\frac{u}{g}\right) = -\frac{1}{2}g\left(\frac{u}{g}\right) ^ 2 + u\left(\frac{u}{g}\right) = \frac{u ^ 2}{2g}$.
    \end{solution}
\end{example}

\subsection{Case \texorpdfstring{$F = F(t)$}{}}
The same method works,
do $\int\,dt$ twice.

\begin{example}
    A particle of mass $m = 1$ is at rest at $x = 0$.
    A force $F = e ^ {-t}$ is switched on at time $t = 0$.
    Find $x(t)$ for $t > 0$.

    \textit{Note:
    expect $\dot{x} > 0$ and $x > 0$ for $t > 0$
    (since $F > 0$).}

    \begin{solution}
        \[
        \ddot{x} = e ^ {-t} \xrightarrow{\int\,dt} \dot{x} = -e ^ {-t} + 1 \xrightarrow{\int\,dt} x = e ^ {-t} + t - 1.
        \]
    \end{solution}
\end{example}

\subsection{Case \texorpdfstring{$F = F(\dot{x})$}{}}

\begin{remark}
    Here $m\ddot{x} = F(\dot{x})$ second-order non linear differential equation.
\end{remark}

\begin{example}
    A particle of mass $m$ is slowed by a frictional force of magnitude $be ^ {av}$
    ($a$ and $b$ are constant).
    Initial speed $u$.
    What time $T$ does the particle travel for before coming to rest?
    
    \begin{solution}
        The particle either moves to the right or the left,
        the force moves in the opposite direction.

        Choosing the first situation.
        So
        \begin{align*}
            m\frac{dv}{dt} = -be ^ {av} &\implies \int e ^ {av}\,dv = -\frac{b}{m}\int\,dt \\
            \intertext{could use a constant of integration,
            fixed by $v(0) = u$.} \\
            \int e ^ {av}\,dv = -\frac{b}{m}\int\,dt &\implies \int_{u}^{0} e ^ {av}\,dv = -\frac{b}{m}\int_{0}^{T}\,dt \\
            &\implies \left[-\frac{1}{a}e ^ {-av}\right]_{u}^{0} = -\frac{bT}{m} \\
            &\implies T = \frac{m}{ab}\left(1 - e ^ {-au}\right).
        \end{align*}
    \end{solution}
\end{example}

\begin{example}
    A mass $M$ falls downwards under gravity,
    a resistive force $bw$,
    where $w$ is its speed.
    Initially $w(0) = 0$,
    find $w(t)$.
    What is the "least upper bound" of this $w$,
    the terminal speed.

    \begin{solution}
        We could use the $x$ axis pointing up or down.
        Use $x$ as downwards since the motion is downwards.

        Then
        \[
        m\dot{v} = mg - bv
        \]
        where $v$ is the velocity,
        here the velocity $v = w$.
        So
        \[
        m\dot{w} = mg - bw \implies \frac{dw}{dt} = g - \frac{b}{m}w \implies \int\frac{1}{g - \frac{b}{m}w}\,dw = \int\,dt
        \]
        which results in $w(t) = \frac{mg}{b}\left(1 - e ^ {-\frac{bt}{m}}\right)$,
        the terminal speed is
        \[
        \liminfty[t]\frac{mg}{b}\left(1 - e ^ {-\frac{bt}{m}}\right) = \frac{mg}{b}.
        \]
    \end{solution}
\end{example}

\subsection{Case \texorpdfstring{$F = F(x)$}{}}
Here $m\ddot{x} = F(x)$.
If $F(x) = bx + c$
($b$ and $c$ are constant),
then $m\ddot{x} - bx = c$ linear,
the solution is the complementary function $+$ the particular integral.
This doesn't work for $F(x)$ non-linear.
For that think of $v = v(x)$.
Then
\[
m\frac{dv}{dt} = m\frac{d}{dt}v(x(t)) = m\frac{dv}{dx}\cdot\frac{dx}{dt} = m\frac{dv}{dx}v = F(x).
\]
This is a first order separable ODE,
solve to get $v(x)$.
To get $x(t)$,
use $\frac{dx}{dt} = v(x)$ again first order separable.

\begin{example}
    A mass with $m = 2$ moves in a force with $F = 3x ^ 2$,
    initial conditions $x = 1$ and $v = 1$ at $t = 0$.
    What time $T$ does it take to reach $x = 9$?

    \begin{solution}
        \begin{align*}
            2v\frac{dv}{dx} = 3x ^ 2 &\implies \int 2v\,dv = \int 3x ^ 2\,dx \\
            &\implies v ^ 2 = x ^ 3 + c &\text{($c = 0$ from initial conditions)} \\
            &\implies v ^ 2 = x ^ 3 \\
            &\implies v = x ^ {\frac{3}{2}} &\text{(positive since $x = v = 1$ at $t = 0$)}
        \end{align*}
        Now
        \begin{align*}
            \frac{dx}{dt} = x ^ {\frac{3}{2}} &\implies \int_{1}^{9} x ^ {-\frac{3}{2}}\,dx = \int_{0}^{T}\,dt \\
            &\implies T = \left[-2x ^ {-\frac{1}{2}}\right]_{2}^{9} = -2\left(\frac{1}{3} - 1\right) = \frac{4}{3}.
        \end{align*}
    \end{solution}
\end{example}

\subsection{More Examples}

\begin{example}
    $F(t, v) = -v + e ^ {-t}$
    (with $v(0) = 0$)
    \begin{solution}
        This is linear,
        so solve with an integrating factor and apply the initial conditions to get
        \[
        v(t) = te ^ {-t}.
        \]
    \end{solution}
\end{example}

\begin{example}
    A rocket of mass $m(t)$ burns fuel at a constant rate $\dot{m} = -c$
    (with $c > 0$).
    Thus produces a constant force $F = kc$.
    Start with $x(0) = 0$ and $\dot{x}(0) = 0$,
    and initial mass $m_0$.
    Find $\dot{x}(t)$,
    hence $x(t)$.
    \begin{solution}
        Here the equation of motion $\frac{d}{dt}(mv) = F$ where $v = \dot{x}$.
        Do $\int\,dt$ giving $mv = kct + 0$
        (with $0$ being the constant of integration).
        Also $\dot{m} = -c \implies m(t) = -ct + m_0$.
        Thus $v(t) = \frac{kct}{m_0 - ct}$ for $0 \leq t < \frac{m_0}{c}$.

        Finally,
        $x(t) = \int v(t)\,dt$.
    \end{solution}
\end{example}

Two methods for $F = F(\dot{x})$.

\textbf{Method $1$}
is $m\frac{dv}{dt} = F(v)$,
get $v(t)$,
then $\int\,dt$ gives $x(t)$.

\textbf{Method $2$}
is $mv\frac{dv}{dx} = F(v)$ which is separable,
get $v(x)$,
then $\frac{dx}{dt} = v(x)$.

\begin{example}
    A unit mass
    (meaning $m = 1$)
    experiences a frictional force of magnitude $v + v ^ 2$
    ($v > 0$ is velocity).
    Find the general solution for $x(t)$.

    \begin{solution}
        Here method $2$ says
        \begin{align*}
            v\frac{dv}{dx} = -(v + v ^ 2) &\implies \frac{dv}{dx} = -(1 + v) \\
            &\implies \int\frac{1}{1 + v}\,dv = -\int\,dx \\
            &\implies \log(1 + v) = -x + C \\
            &\implies v(x) = e ^ {c - x} - 1.
        \end{align*}

        Then
        \begin{align*}
            \frac{dx}{dt} = v = e ^ {c - x} - 1 &\implies \int\frac{1}{e ^ {c - x} - 1}\,dx = \int\,dt = t + b \\
            &\implies \int\frac{e ^ x}{e ^ c - e ^ x}\,dx = -\log(e ^ c - e ^ x) = t + b \\
            &\implies -\log(e ^ c - e ^ x) = t + b \\
            &\implies e ^ c - e ^ x = e ^ {-b - b} \\
            &\implies x = \log(e ^ c - e ^ {-b - t}).
        \end{align*}
    \end{solution}
\end{example}

\begin{example}
    A unit mass is acted on by a force $F = \frac{1}{1 + x ^ 2}$,
    "starts" at $x = -\infty$ with $\dot{x} = u_0 > 0$.
    What is $\dot{x}$ as $x \rightarrow \infty$?

    \textit{[Note:
    $F > 0$ so we expect an answer $> u_0$.]}
    \begin{solution}
        We really want $v(x)$.
        The equation is
        \begin{align*}
            v\frac{dv}{dx} = \frac{1}{1 + x ^ 2} &\implies \int_{u_0}^{u_1} v\,dv = \int_{-\infty}^{\infty}\frac{1}{1 + x ^ 2}\,dx \\
            &\implies \frac{1}{2}u_1 ^ 2 - \frac{1}{2}u_0 ^ 2 = \left[\arctan{x}\right]_{-\infty}^{\infty} = \frac{\pi}{2} - \left(-\frac{\pi}{2}\right) = \pi \\
            &\implies u_1 ^ 2 = u_0 ^ 2 + 2\pi \\
            &\implies u_1 = \sqrt{u_0 ^ 2 + 2\pi}\qquad(> u_0\text{ as expected}).
        \end{align*}
    \end{solution}
\end{example}

Define $V(x) = -\int F(x)\,dx$.
Then
\[
\frac{d}{dx}\left(\frac{1}{2}mv ^ 2\right) = m\frac{dv}{dx}v = F = -\frac{d}{dx}V
\]
so $\frac{d}{dx}\left(\frac{1}{2}mv ^ 2 + V\right) = 0 \implies \frac{1}{2}mv ^ 2 + V(x) = E$.
This constant $E$ is the
(total)
energy,
while $\frac{1}{2}mv ^ 2$ is kinetic energy and $V(x)$ is potential energy.
Also note $\frac{d}{dt}E = \frac{dE}{dx}\frac{dx}{dt} = 0$,
therefore $E$ is constant in time.
\begin{remark}
    \begin{enumerate}[label = (\roman*)]
        \item We say that $E$ is conserved,
        and the force is conservative.

        \item Can add a constant
        (of integration)
        to $V$,
        and hence to $E$.

        \item Example:
        gravity close to the surface of a planet,
        take $x$ upwards,
        then force is
        \[
        F = -mg \implies V(x) = mgx\quad(+\text{optional constant}).
        \]
        
        \item In cases where one cannot solve for $x(t)$,
        energy arguments can still tell us something.
        See next example.
    \end{enumerate}
\end{remark}

\begin{example}
    Take $m = 2$ and $V(x) = x ^ 6$.
    So
    \[
    E = \frac{1}{2}mv ^ 2 + V(x) = \dot{x} ^ 2 + x ^ 6.
    \]
    Try to find $x(t)$ by
    \[
    \frac{dx}{dt} = \sqrt{E - x ^ 6} \implies \int\frac{1}{\sqrt{E - x ^ 6}}\,dx = \int\,dt.
    \]
    Note $V(x) \leq E$ restricting $x$ to say initial conditions $x(0) = 0, \dot{x}(0) = 1$.
    So $E = 1 ^ 6 + 0 ^ 6 = 1$ at $t = 0$,
    therefore for all $t$.
    Thus $-1 \leq x(t) \leq 1$.
    Think of a bowl,
    gravity acting downwards,
    particle rolls in it
    (just an analogy).

    Now $x$ increases to $1$,
    turns around and decreases,
    passes $x = 0$ and "rolls up" the other side,
    reaches $x = -1$,
    turns round,
    etc.
    Motion is periodic.

    Can we compute the period $P$
    (time to complete one cycle)?
    No,
    however
    \[
    \int\frac{1}{\sqrt{1 - x ^ 6}}\,dx,
    \]
    can't do that.
\end{example}

\begin{definition}
    An equilibrium point is where force is $0$,
    i.e. $\frac{dV}{dx} = 0$.
\end{definition}

In the above example,
one equilibrium point at $x = 0$.
(Particle at rest at such a point will stay there.)

\subsection{Motion in a potential}

\begin{example}
    Particle of mass $m = 3$ in a potential $V(x) = \frac{1}{4}x ^ 4 - \frac{1}{3}x ^ 3 - x ^ 2$.
    Describe the motion.

    Draw a graph of $V$.
    Compute $\frac{dV}{dx} = x ^ 3 - x ^ 2 - 2x = x(x ^ 2 - x - 2) = x(x - 2)(x + 1)$.
    So there are three equilibrium points $x = 0, 2, -1$.

    Need enough energy to get over the "hill" at $x = 0$.
    Initial direction doesn't matter.
    The equation is something like
    \[
    E = \frac{1}{2}mu ^ 2 + V(1) = \text{tiny bit} + V(0).
    \]
    Thus $\frac{1}{2}mu ^ 2 + V(1) > V(0)$.
    \[
    \frac{3}{2}u ^ 2 - \frac{13}{12} > 0 \iff u > \sqrt{\frac{13}{18}}.
    \]
\end{example}

\subsection{Simple Harmonic Motion}
Usually a mass-spring system,
restoring force $F = -kx$ where $k > 0$ is the spring constant.
This $F$ is a conservative,
and $V(x) = -\int F\,dx = \frac{1}{2}kx ^ 2$.
Equation of motion is $m\ddot{x} = -kx \implies m\ddot{x} + kx = 0$,
general solution $x(t) = A\cos(\omega t) + B\sin(\omega t)$,
where $\omega = \sqrt{\frac{k}{m}}$ and $A$ and $B$ are arbitrary constants.
Here $\omega$ is the angular frequency,
and the period is $p = \frac{2\pi}{\omega}$.

Variant:
spring hangs downwards,
under gravity.
Now
\[
m\ddot{x} = -kx - mg,
\]
and
\[
x(t) = A\cos(\omega t) + B\sin(\omega t) - \frac{mg}{k}.
\]
The effect is to shift the equilibrium by an amount $\frac{mg}{k}$.

\subsection{Damping}
Car suspension,
each wheel has a spring,
and also a shock absorber,
which provides damping.
Has the form $-(\text{positive constant})\dot{x}$ so opposes velocity.
No longer have a conserved energy.
The equation is
\[
m\ddot{x} = -kx - 2mb\dot{x}
\]
with $b > 0$ constant\footnote{The $2mb$ is just for convenience,
it can be any constant.}.

Auxiliary equation
\begin{align*}
    m\lambda ^2 + 2mb\lambda + k = 0 &\implies \lambda ^ 2 + 2b\lambda + \frac{k}{m} = 0 \\
    &\implies \lambda ^ 2 + 2b\lambda + \omega ^ 2 = 0.
\end{align*}
Roots
\[
\lambda_{\pm} = -b \pm \sqrt{b ^ 2 - \omega ^ 2}
\]
so
\[
x(t) = Ae ^ {\lambda_{+}t} + Be ^ {\lambda_{-}t}.
\]
Case when $b > \omega \implies \lambda_{\pm}$ real,
both negative.
Any initial $x$ dies out exponentially fast.
This is called over damping.
No oscillation at all.

\subsection{Small oscillations}
If $V'(x_0) = 0$ then $x_0$ is an equilibrium point,
where $F(x_0) = 0$.
It is a stable equilibrium if it is a local minimum,
i.e. $V''(x_0) > 0$.
Otherwise unstable,
$V''(x_0) < 0$.
Then the period of small oscillations about a stable equilibrium is the period of the best fitting simple harmonic oscillator.
Computing $P$.
Let $x_0$ be a local minimum of $V(x)$.
Write $x(t) = x_0 + \epsilon(t)$ where $\epsilon(t)$ is a small function.
Substitute into equation of motion
\[
m\ddot{x} = F(x) = -V'(x) \implies m\ddot{\epsilon} = F(x_0 + \epsilon) = \underbrace{F(x_0)}_{=0} + \epsilon F'(x_0) + \dotsc
\]
\[
\implies m\ddot{\epsilon} \approx \epsilon F'(x_0) = -V''(x_0)\epsilon.
\]
This is the equation for simple harmonic motion,
where $V''(x_0)$ is the "spring constant" $k$.
So the period of small oscillations is $P = 2\pi\sqrt{\frac{m}{V''(x)}}$.
Makes sense for local minimum where $V''(x_0) > 0$.

\begin{example}
    $m = 3$,
    $V(x) = \frac{1}{4}x ^ 4 - \frac{1}{3}x ^ 3 - x ^ 2$.
    Then $V'(x) = x(x + 1)(x - 2)$,
    $x = 0$ is unstable,
    $x = -1, 2$ are stable.
    Look for period $P$ about $x = -1$.
    $V''(x) = \frac{d}{dx}\left[x(x + 1)(x - 2)\right]$,
    so $V''(-1) = \left. x(x - 2)\right|_{x = -1} = 3$,
    hence $P = 2\pi\sqrt{\frac{m}{V''(x_0)}} = 2\pi\sqrt{\frac{3}{3}} = 2\pi$.
\end{example}

\subsection{Conservation of Momentum}
Here the external force is $0$.

Fact:
the total momentum is conserved by collisions.
Total momentum is the sum of the momenta of each particle.
The total momentum after the collision is equal to the total momentum before the collision.
The total energy
(which is all kinetic energy)
may be conserved
(then the collision was elastic)
or not conserved
(the collision was inelastic).

\section{}


\subsection{Charged particle in electromagnetic field}

\begin{definition}
    An electric field is a vector $\mbf{E}$
    (in general function of $x, y, z, t$ but we will take it constant).
\end{definition}

Similarly magnetic field $\mbf{B}$.

A particle of charge $q$ experiences the Lorentz force.
\[
\mbf{F} = q\mbf{E} + q\mbf{v} \times \mbf{B}
\]
where $\mbf{v}$ is velocity of particle.

Convention:
$\mbf{e}_1 \times \mbf{e}_2 = \mbf{e}_3$,
$\mbf{e}_2 \times \mbf{e}_3 = \mbf{e}_1$,
$\mbf{e}_3 \times \mbf{e}_1 = \mbf{e}_2$,
$\mbf{e}_2 \times \mbf{e}_1 = -\mbf{e}_3$ etc.

\begin{example}
    Take $\mbf{E} = \mbf{0}$ and $\mbf{B} = B\mbf{e}_3$ with $B$ constant.
    Initial conditions $\mbf{r}(0) = \mbf{0}$ and $\dot{\mbf{r}} = u\mbf{e}_1$.
    Find $\mbf{r}(t)$.

    \begin{solution}
        Equation of motion $m\ddot{\mbf{r}} = \mbf{F} = q\dot{\mbf{r}} \times \mbf{B} = qB \dot{\mbf{r}} \times \mbf{e}_3$.

        Do $\int\,dt$ to get $m\dot{\mbf{r}} = qB\mbf{r} \times \mbf{e}_3 + \underbrace{mu\mbf{e}_1}_{\text{constant of integration}}$.
        Write $\mbf{r} = x\mbf{e}_1 + y\mbf{e}_2 + z\mbf{e}_3$,
        then
        \begin{align*}
            m\dot{x} &= mu + qBy \\
            m\dot{y} &= -qBx \\
            m\dot{z} &= 0
        \end{align*}
        so $z(t) = 0$ solves for $z$.
        Left with two coupled equations for $x$ and $y$.
        Eliminate $x$ or $y$
        (either):
        say $y$.
        Namely $m\ddot{x} = qB\dot{y} = -\left(\frac{qB}{m}\right)x(qB) \implies \ddot{x} + \left(\frac{qB}{m}\right) ^ 2x = 0$.

        General solution is $x(t) = \alpha\cos(\omega t) + \beta\sin(\omega t)$,
        $\alpha, \beta$ constants,
        $\omega = \frac{qB}{m}$.
        And $x(0) = 0 \implies \alpha = 0$ so $x(t) = \beta\sin(\omega t)$.
        And $\dot(0) = u \implies \beta\omega = u \implies \beta = \frac{\omega}{u}$.
        Finally the first equation implies $y = \frac{m}{qB}(\dot{x} - u) = \frac{mu}{qB}(1 - \cos(\omega t)) = \frac{u}{\omega}(1 - \cos(\omega t))$.
    \end{solution}
\end{example}

\begin{example}
    As before,
    with $m = q = 1$,
    and an electric field $\mbf{E} = E\mbf{e}_2$ with $E$ constant.

    \begin{solution}
        $\ddot{\mbf{r}} = B\dot{\mbf{r}} \times \mbf{e}_3 + E\mbf{e}_2$.

        \[
        \int\,dt \implies \dot{\mbf{r}} = B\mbf{r} \times \mbf{e}_3 + Et\mbf{e}_2 + u\mbf{e}_1.
        \]
        $z(t) = 0$ for all $t$ since no vector points in direction $\mbf{e}_3$.
        \begin{align*}
            \dot{x} &= u + By \\
            \dot{y} &= -Bx + Et.
        \end{align*}
        Eliminate $y$:
        $\ddot{x} = B\dot{y} = -B ^ 2x + EBt \implies \ddot{x} + B ^ 2x = EBt$.
        Complementary function is $x = \alpha\cos(Bt) + \beta\sin(Bt)$,
        particular integral $x_{PI} = \frac{E}{B}t$.
        Etc.
        
    \end{solution}
\end{example}































\end{document}